Adapt Datatypes

HOL_To_IMP_Minus/Refinements/HOL_To_IMP_Minus_Datatypes.thy
@@ -21,10 +21,6 @@ thm Pair_nat_def
 compile_nat Pair_nat_def
 HOL_To_IMP_Minus_correct Pair_nat by cook
 
-(* Problem: We have obtained an unconditional equation. However, we
-still have to prove it to be related to the original HOL function.
-TODO: how to prove the two functions to be related? Currently, we are
-missing the right lemmas to make it automatic. *)
 context
   fixes xs and xs' :: "'a :: compile_nat * 'b :: compile_nat"
   assumes rels: "Rel_nat xs xs'"
@@ -94,9 +90,14 @@ and the thm is not found
 *)
 
 HOL_To_IMP_Minus_correct HOL_To_HOL_Nat.rev_acc_nat
-  sorry
+  oops
 
-lemma
+(* Findings:
+ - For introduction over multiple variable we need to apply the search for
+    contradiction multiple times
+ - Problem mit if-placement siehe count_acc Beispiel *)
+
+lemma rev_acc_cor:
   assumes "Rel_nat (s ''rev_acc_nat.args.x'') (x :: 'a list)"
   assumes "Rel_nat (s ''rev_acc_nat.args.xa'') (xa :: 'a list)"
   shows "terminates_with_res_IMP_Minus (tailcall_to_IMP_Minus rev_acc_nat_IMP_tailcall) s ''rev_acc_nat.ret''
@@ -143,132 +144,10 @@ lemma
   apply (subst case_list_nat_def)
   apply (split if_splits; intro impI conjI; simp)
   (*apply IH; prove side-conditions*)
-  oops
-
-  thm HTHN.rev_acc_nat_eq_unfolded
-  thm Rel_nat_destruct_Cons_nat
-
-
-lemma fst_nat_natify_Nil: "fst_nat (natify []) = 0"
-  by (simp add: Nil_nat_def natify_list.simps)
-lemma fst_nat_natify_Cons: "fst_nat (natify (x#xs)) = 1"
-  by (simp add: Cons_nat_def natify_list.simps)
-
-thm HTHN.rev_acc.induct
-lemma
-  assumes "s ''rev_acc_nat.args.x'' = natify x"
-    and   "s ''rev_acc_nat.args.xa'' = natify xa"
-   shows  "terminates_with_res_IMP_Minus (tailcall_to_IMP_Minus rev_acc_nat_IMP_tailcall) s
-     ''rev_acc_nat.ret''
-     (natify (HTHN.rev_acc x xa))"
-  using assms apply -
-  apply (tactic \<open>HM.correct_if_IMP_tailcall_correct_tac HT.get_IMP_def @{context} 1\<close>)
-proof (induction x xa arbitrary: s rule: HTHN.rev_acc.induct)
-  case (1 acc)
-  show ?case apply -
-    apply (rule terminates_with_res_IMP_Tailcall_start)
-    apply (subst (2) rev_acc_nat_IMP_tailcall_def)
-    apply (tactic \<open>HT.run_step_tac HT.get_imp_minus_correct @{context} 1\<close>)
-    apply (tactic \<open>HT.run_step_tac HT.get_imp_minus_correct @{context} 1\<close>)
-    apply (tactic \<open>HT.run_step_tac HT.get_imp_minus_correct @{context} 1\<close>)
-    apply (tactic \<open>HT.run_step_tac HT.get_imp_minus_correct @{context} 1\<close>)
-    apply (tactic \<open>HT.run_step_tac HT.get_imp_minus_correct @{context} 1\<close>)
-    apply (tactic \<open>HT.run_step_tac HT.get_imp_minus_correct @{context} 1\<close>)
-    apply (tactic \<open>HT.run_step_tac HT.get_imp_minus_correct @{context} 1\<close>)
-    apply (tactic \<open>HT.run_step_tac HT.get_imp_minus_correct @{context} 1\<close>)
-    apply (tactic \<open>HT.run_step_tac HT.get_imp_minus_correct @{context} 1\<close>)
-    using 1 apply -
-     apply (tactic \<open>HT.finish_non_tail_tac @{context} 1\<close>)
-    by (simp add: fst_nat_natify_Nil 1)
-next
-  case (2 x xs acc)
-  (* Ugly but quite helpful *)
-  let ?S = "(STATE (interp_state (update_state (update_state (update_state (update_state (update_state (update_state (update_state (update_state (update_state (update_state (update_state (update_state (update_state (update_state (update_state (update_state (update_state (update_state (update_state (update_state (update_state (State s)
-        ''.args.0'' (s ''rev_acc_nat.args.x'')) ''.args.1'' (s ''rev_acc_nat.args.xa'')) ''fst_nat.args.m'' (s ''rev_acc_nat.args.x''))
-        ''fst_nat.ret'' (fst_nat (s ''rev_acc_nat.args.x''))) ''eq.args.x'' (fst_nat (s ''rev_acc_nat.args.x''))) ''eq.args.y'' 0)
-        ''eq.ret'' (natify (fst_nat (s ''rev_acc_nat.args.x'') = 0))) ''.If.7'' (natify (fst_nat (s ''rev_acc_nat.args.x'') = 0)))
-        ''snd_nat.args.m'' (s ''rev_acc_nat.args.x'')) ''snd_nat.ret'' (snd_nat (s ''rev_acc_nat.args.x''))) ''snd_nat.args.m'' (snd_nat (s ''rev_acc_nat.args.x'')))
-        ''snd_nat.ret'' (snd_nat (snd_nat (s ''rev_acc_nat.args.x'')))) ''rev_acc_nat.args.x'' (snd_nat (snd_nat (s ''rev_acc_nat.args.x''))))
-        ''snd_nat.args.m'' (s ''rev_acc_nat.args.x'')) ''snd_nat.ret'' (snd_nat (s ''rev_acc_nat.args.x''))) ''fst_nat.args.m'' (snd_nat (s ''rev_acc_nat.args.x'')))
-        ''fst_nat.ret'' (fst_nat (snd_nat (s ''rev_acc_nat.args.x''))))
-        ''Cons_nat.args.x'' (fst_nat (snd_nat (s ''rev_acc_nat.args.x'')))) ''Cons_nat.args.xa'' (s ''rev_acc_nat.args.xa'')) ''Cons_nat.ret'' (Cons_nat (fst_nat (snd_nat (s ''rev_acc_nat.args.x''))) (s ''rev_acc_nat.args.xa'')))
-        ''rev_acc_nat.args.xa'' (Cons_nat (fst_nat (snd_nat (s ''rev_acc_nat.args.x''))) (s ''rev_acc_nat.args.xa'')))))"
-  have x: "?S ''rev_acc_nat.args.x'' = natify xs"
-    using 2(2) by (auto simp: STATE_interp_update_retrieve_key_eq_if Cons_nat_def natify_list.simps)
-  have xa: "?S ''rev_acc_nat.args.xa'' = natify (x#acc)"
-    using 2
-    by (simp add: STATE_interp_update_retrieve_key_eq_if Cons_nat_def natify_list.simps)
-  show ?case apply -
-    apply (rule terminates_with_res_IMP_Tailcall_start)
-    apply (subst (2) rev_acc_nat_IMP_tailcall_def)
-    apply (tactic \<open>HT.run_step_tac HT.get_imp_minus_correct @{context} 1\<close>)
-    apply (tactic \<open>HT.run_step_tac HT.get_imp_minus_correct @{context} 1\<close>)
-    apply (tactic \<open>HT.run_step_tac HT.get_imp_minus_correct @{context} 1\<close>)
-    apply (tactic \<open>HT.run_step_tac HT.get_imp_minus_correct @{context} 1\<close>)
-    apply (tactic \<open>HT.run_step_tac HT.get_imp_minus_correct @{context} 1\<close>)
-    apply (tactic \<open>HT.run_step_tac HT.get_imp_minus_correct @{context} 1\<close>)
-    apply (tactic \<open>HT.run_step_tac HT.get_imp_minus_correct @{context} 1\<close>)
-    apply (tactic \<open>HT.run_step_tac HT.get_imp_minus_correct @{context} 1\<close>)
-    apply (tactic \<open>HT.run_step_tac HT.get_imp_minus_correct @{context} 1\<close>)
-    apply (simp add: fst_nat_natify_Cons 2)
-    apply (tactic \<open>HT.run_step_tac HT.get_imp_minus_correct @{context} 1\<close>)
-    apply (tactic \<open>HT.run_step_tac HT.get_imp_minus_correct @{context} 1\<close>)
-    apply (tactic \<open>HT.run_step_tac HT.get_imp_minus_correct @{context} 1\<close>)
-    apply (tactic \<open>HT.run_step_tac HT.get_imp_minus_correct @{context} 1\<close>)
-    apply (tactic \<open>HT.run_step_tac HT.get_imp_minus_correct @{context} 1\<close>)
-    apply (tactic \<open>HT.run_step_tac HT.get_imp_minus_correct @{context} 1\<close>)
-    apply (tactic \<open>HT.run_step_tac HT.get_imp_minus_correct @{context} 1\<close>)
-    apply (tactic \<open>HT.run_step_tac HT.get_imp_minus_correct @{context} 1\<close>)
-    apply (tactic \<open>HT.run_step_tac HT.get_imp_minus_correct @{context} 1\<close>)
-    apply (tactic \<open>HT.run_step_tac HT.get_imp_minus_correct @{context} 1\<close>)
-    apply (tactic \<open>HT.run_step_tac HT.get_imp_minus_correct @{context} 1\<close>)
-    apply (tactic \<open>HT.run_step_tac HT.get_imp_minus_correct @{context} 1\<close>)
-    apply (tactic \<open>HT.run_step_tac HT.get_imp_minus_correct @{context} 1\<close>)
-    using 2(1)[of ?S, OF x xa]
-    by (simp add: terminates_with_res_tTailI)
-qed
-
-end
-
-context HOL_To_HOL_Nat
-begin
-
-lemma rev_eq_rev_acc_nil: "List.rev xs = rev_acc xs []" by simp
-
-end
-
-experiment
-begin
-interpretation HOL_To_HOL_Nat .
-function_compile_nat rev_eq_rev_acc_nil
-(*We couldn't use 'unconditional_nat' this way since the synthesised definition uses an auxiliary
-function (rev_acc_nat) with TYPE('a) arguments.*)
-print_statement rev_nat_eq_unfolded
-end
-
-context HOL_To_HOL_Nat
-begin
-
-(*we can fix this by registering the relatedness theorem of the unconditional rev_acc_nat function
-to transfer instead*)
-declare HNTIM.related_rev_acc_nat_unconditional[transfer_rule]
-  and rev_acc_related_transfer[transfer_rule del] (*deletion is optional*)
-function_compile_nat rev_eq_rev_acc_nil
-print_statement rev_nat_eq_unfolded
-end
-
-context HOL_Nat_To_IMP_Minus
-begin
-
-unconditional_nat HTHN.rev_nat_eq_unfolded
-declare rev_nat_unconditional.simps[simp del]
-compile_nat rev_nat_unconditional.simps
-HOL_To_IMP_Minus_correct rev_nat_unconditional by cook
-
-(*TODO: derive these theorems automatically*)
-lemma related_rev_nat_unconditional [transfer_rule]:
-  "(Rel_nat ===> Rel_nat) rev_nat_unconditional rev"
   sorry
+
+HOL_To_IMP_Minus_correct HOL_To_HOL_Nat.rev_acc_nat
+  using rev_acc_cor by blast
 
 end
 
@@ -292,84 +171,56 @@ context HOL_Nat_To_IMP_Minus
 begin
 
 lemmas length_acc_nat_eq = HTHN.length_acc_nat_eq_unfolded[simplified case_list_nat_def]
-unconditional_nat length_acc_nat_eq
-declare length_acc_nat_unconditional.simps[simp del]
-compile_nat length_acc_nat_unconditional.simps
-HOL_To_IMP_Minus_correct length_acc_nat_unconditional by (cook mode = tailcall)
+compile_nat length_acc_nat_eq
+HOL_To_IMP_Minus_correct HOL_To_HOL_Nat.length_acc_nat
+  oops
 
-lemma related_length_acc_nat_unconditional [transfer_rule]:
-  "(Rel_nat ===> Rel_nat ===> Rel_nat) length_acc_nat_unconditional HTHN.length_acc"
+lemma "Rel_nat (s ''length_acc_nat.args.x'') (y::'a list) \<Longrightarrow>
+       Rel_nat (s ''length_acc_nat.args.xa'') (ya::nat) \<Longrightarrow>
+    terminates_with_res_IMP_Minus (tailcall_to_IMP_Minus length_acc_nat_IMP_tailcall)
+      s ''length_acc_nat.ret''
+     (HTHN.length_acc_nat TYPE('a::compile_nat) (s ''length_acc_nat.args.x'') (s ''length_acc_nat.args.xa''))"
+  apply (rule terminates_with_res_IMP_Minus_if_terminates_with_res_IMP_TailcallI)
+    apply (subst length_acc_nat_IMP_tailcall_def; simp)
+  apply (subst length_acc_nat_IMP_tailcall_def; simp)
+  apply (induction "y" "ya" arbitrary: s rule: HTHN.length_acc.induct)
+  (*case []*)
+  apply (subst (2) length_acc_nat_IMP_tailcall_def, rule terminates_with_res_IMP_Tailcall_start)
+   apply (tactic \<open>HT.run_step_tac HT.get_imp_minus_correct @{context} 1\<close>)+
+    (*check the retrieved condition for a contradiction (needs to be built into the IF tactic*)
+    apply (erule check_first_nat_ccontradictionE check_first_nat_ccontradictionE')
+    apply (rule fst_nat_eq_if_Rel_nat_list)
+    apply assumption (*needs a smarter method*)
+    apply simp
+  apply (subst HTHN.length_acc_nat_eq_unfolded)
+  apply (assumption, assumption)
+  apply (subst case_list_nat_def)
+  apply (split if_splits; intro impI conjI; simp)
+  apply (tactic \<open>HT.finish_non_tail_tac @{context} 1\<close>)
+    (*we need to derive a contradiction*)
+    apply (erule check_first_nat_ccontradictionE check_first_nat_ccontradictionE')
+    apply (rule fst_nat_eq_if_Rel_nat_list)
+    apply assumption
+    apply simp
+  (*case x#xs*)
+  apply (subst (2) length_acc_nat_IMP_tailcall_def, rule terminates_with_res_IMP_Tailcall_start)
+  apply (tactic \<open>HT.run_step_tac HT.get_imp_minus_correct @{context} 1\<close>)+
+    (*we need to derive a contradiction*)
+    apply (erule check_first_nat_ccontradictionE check_first_nat_ccontradictionE')
+    apply (rule fst_nat_eq_if_Rel_nat_list)
+    apply assumption
+    apply simp
+    (*check the retrievied condition for a contradiction*)
+    apply (erule check_first_nat_ccontradictionE check_first_nat_ccontradictionE')
+    apply (rule fst_nat_eq_if_Rel_nat_list)
+    apply assumption
+    apply simp
+  apply (tactic \<open>HT.run_step_tac HT.get_imp_minus_correct @{context} 1\<close>)+
+  apply (subst HTHN.length_acc_nat_eq_unfolded)
+  apply (assumption, assumption)
+  apply (subst case_list_nat_def)
+  apply (split if_splits; intro impI conjI; simp)
   sorry
-
-end
-
-context HOL_To_HOL_Nat
-begin
-
-(*introduce a definition because List.length is just an abbreviation*)
-definition length where "length xs \<equiv> length_acc xs 0"
-
-lemma length_eq_length [simp]: "length = List.length"
-  unfolding length_def by simp
-
-declare HNTIM.related_length_acc_nat_unconditional[transfer_rule]
-function_compile_nat length_def
-
-end
-
-context HOL_Nat_To_IMP_Minus
-begin
-
-unconditional_nat HTHN.length_nat_eq_unfolded
-declare length_nat_unconditional.simps[simp del]
-compile_nat length_nat_unconditional.simps
-HOL_To_IMP_Minus_correct length_nat_unconditional by cook
-
-lemma related_length_nat_unconditional [transfer_rule]:
-  "(Rel_nat ===> Rel_nat) length_nat_unconditional length"
-  sorry
-
-end
-
-context HOL_To_HOL_Nat
-begin
-
-lemma append_eq_rev_acc_rev: "List.append xs ys = rev_acc (rev xs) ys"
-  by simp
-
-(*for some reason, transfer needs the lemma below instead of the existing, point-free version to
-synthesise the right definition*)
-(* declare HNTIM.related_rev_nat_unconditional[transfer_rule] *)
-
-lemma related_rev_nat_unconditional [transfer_rule]:
-  assumes "Rel_nat xs ys"
-  shows "Rel_nat (HNTIM.rev_nat_unconditional xs) (rev ys)"
-  by (fact rel_funD[OF HNTIM.related_rev_nat_unconditional assms])
-
-(* schematic_goal
-  assumes [transfer_rule]: "Rel_nat f xs"
-  assumes [transfer_rule]: "Rel_nat g ys"
-  shows "Rel_nat
-    (HNTIM.rev_acc_nat_unconditional (HNTIM.rev_nat_unconditional f) g)
-    (rev_acc (rev xs) ys)"
-  by transfer_prover *)
-
-function_compile_nat append_eq_rev_acc_rev
-
-end
-
-context HOL_Nat_To_IMP_Minus
-begin
-
-unconditional_nat HTHN.append_nat_eq_unfolded
-declare append_nat_unconditional.simps[simp del]
-compile_nat append_nat_unconditional.simps
-HOL_To_IMP_Minus_correct append_nat_unconditional by cook
-
-lemma related_append_nat_unconditional [transfer_rule]:
-  "(Rel_nat ===> Rel_nat ===> Rel_nat) append_nat_unconditional append"
-  sorry
-
 end
 
 context HOL_To_HOL_Nat
@@ -393,44 +244,227 @@ context HOL_Nat_To_IMP_Minus
 begin
 
 lemmas zip_acc_nat_eq = HTHN.zip_acc_nat_eq_unfolded[simplified case_list_nat_def]
-unconditional_nat zip_acc_nat_eq
-declare zip_acc_nat_unconditional.simps [simp del]
-compile_nat zip_acc_nat_unconditional.simps
-HOL_To_IMP_Minus_correct zip_acc_nat_unconditional by (cook mode = tailcall)
-
-lemma related_zip_acc_nat_unconditional [transfer_rule]:
-  "(Rel_nat ===> Rel_nat ===> Rel_nat ===> Rel_nat) zip_acc_nat_unconditional HTHN.zip_acc"
+compile_nat zip_acc_nat_eq
+HOL_To_IMP_Minus_correct HOL_To_HOL_Nat.zip_acc_nat
   sorry
 
+lemma "Rel_nat (s ''zip_acc_nat.args.x'') (y::'a list) \<Longrightarrow>
+    Rel_nat (s ''zip_acc_nat.args.xa'') (ya::'b list) \<Longrightarrow>
+    Rel_nat (s ''zip_acc_nat.args.xb'') (yb::('a * 'b) list) \<Longrightarrow>
+    terminates_with_res_IMP_Minus (tailcall_to_IMP_Minus zip_acc_nat_IMP_tailcall)
+      s ''zip_acc_nat.ret''
+     (HTHN.zip_acc_nat TYPE('a::compile_nat) TYPE('b::compile_nat)
+       (s ''zip_acc_nat.args.x'') (s ''zip_acc_nat.args.xa'') (s ''zip_acc_nat.args.xb''))"
+  apply (rule terminates_with_res_IMP_Minus_if_terminates_with_res_IMP_TailcallI)
+   apply (subst zip_acc_nat_IMP_tailcall_def; simp)
+   apply (subst zip_acc_nat_IMP_tailcall_def; simp)
+  apply (induction y ya yb arbitrary: s rule: HTHN.zip_acc.induct)
+  (*case [] _*)
+  apply (subst (2) zip_acc_nat_IMP_tailcall_def, rule terminates_with_res_IMP_Tailcall_start)
+  apply (tactic \<open>HT.run_step_tac HT.get_imp_minus_correct @{context} 1\<close>)+
+    (*check the retrieved condition for a contradiction (needs to be built into the IF tactic*)
+    apply (erule check_first_nat_ccontradictionE check_first_nat_ccontradictionE')
+    apply (rule fst_nat_eq_if_Rel_nat_list)
+    apply assumption (*needs a smarter method*)
+    apply simp
+  apply (subst HTHN.zip_acc_nat_eq_unfolded)
+    apply (assumption, assumption, assumption)
+    apply (subst case_list_nat_def)
+    apply (split if_splits; intro impI conjI; simp)
+    apply (tactic \<open>HT.finish_non_tail_tac @{context} 1\<close>)
+    (*we need to derive a contradiction*)
+    apply (erule check_first_nat_ccontradictionE check_first_nat_ccontradictionE')
+     apply (rule fst_nat_eq_if_Rel_nat_list)
+    apply assumption
+    apply simp
+  (* case _ []*)
+  apply (subst (2) zip_acc_nat_IMP_tailcall_def, rule terminates_with_res_IMP_Tailcall_start)
+   apply (tactic \<open>HT.run_step_tac HT.get_imp_minus_correct @{context} 1\<close>)+
+      (*check first case \<rightarrow> find contradiction*)
+    apply (erule check_first_nat_ccontradictionE check_first_nat_ccontradictionE')
+    apply (rule fst_nat_eq_if_Rel_nat_list)
+    apply assumption (*needs a smarter method*)
+    apply simp
+   apply (tactic \<open>HT.run_step_tac HT.get_imp_minus_correct @{context} 1\<close>)+
+    apply (erule check_first_nat_ccontradictionE check_first_nat_ccontradictionE')
+    apply (rule fst_nat_eq_if_Rel_nat_list)
+     apply assumption (*needs a smarter method*)
+  subgoal for v
+    sorry
+
+    (* Need to apply the search for contradiction multiple times ! *)
+    apply (erule check_first_nat_ccontradictionE check_first_nat_ccontradictionE')
+    apply (rule fst_nat_eq_if_Rel_nat_list)
+    apply assumption
+    apply (erule check_first_nat_ccontradictionE check_first_nat_ccontradictionE')
+    apply (rule fst_nat_eq_if_Rel_nat_list)
+    apply assumption
+    apply simp
+  
+  (*case x#xs*)
+  apply (subst (2) zip_acc_nat_IMP_tailcall_def, rule terminates_with_res_IMP_Tailcall_start)
+  apply (tactic \<open>HT.run_step_tac HT.get_imp_minus_correct @{context} 1\<close>)+
+    (*we need to derive a contradiction*)
+    apply (erule check_first_nat_ccontradictionE check_first_nat_ccontradictionE')
+    apply (rule fst_nat_eq_if_Rel_nat_list)
+    apply assumption
+    apply simp
+  apply (tactic \<open>HT.run_step_tac HT.get_imp_minus_correct @{context} 1\<close>)+
+    (*check the retrievied condition for a contradiction*)
+    apply (erule check_first_nat_ccontradictionE check_first_nat_ccontradictionE')
+    apply (rule fst_nat_eq_if_Rel_nat_list)
+    apply assumption
+    apply (erule check_first_nat_ccontradictionE check_first_nat_ccontradictionE')
+    apply (rule fst_nat_eq_if_Rel_nat_list)
+    apply assumption
+    apply simp
+  apply (tactic \<open>HT.run_step_tac HT.get_imp_minus_correct @{context} 1\<close>)+
+    subgoal for v
+      sorry
+    done
+
 end
+
 
 context HOL_To_HOL_Nat
 begin
 
-lemma zip_eq_rev_zip_acc_nil: "List.zip xs ys = rev (zip_acc xs ys [])"
-  by simp
+fun count_acc :: "'a \<Rightarrow> 'a list \<Rightarrow> nat \<Rightarrow> nat" where
+  "count_acc a [] n = n"
+| "count_acc a (x#xs) n = (if x = a then count_acc a xs (Suc n) else count_acc a xs n)"
+declare count_acc.simps[simp del]
 
-(*TODO: why is this needed?*)
-declare
-  HNTIM.related_zip_acc_nat_unconditional[THEN rel_funD, THEN rel_funD, THEN rel_funD,transfer_rule]
-
-(*TODO: something is quite slow here*)
-function_compile_nat zip_eq_rev_zip_acc_nil
+case_of_simps count_acc_eq : count_acc.simps
+function_compile_nat count_acc_eq
 
 end
 
 context HOL_Nat_To_IMP_Minus
 begin
 
-unconditional_nat HTHN.zip_nat_eq_unfolded
-declare zip_nat_unconditional.simps [simp del]
-compile_nat zip_nat_unconditional.simps
-HOL_To_IMP_Minus_correct zip_nat_unconditional by cook
+lemmas count_acc_nat_eq = HTHN.count_acc_nat_eq_unfolded[simplified case_list_nat_def]
+compile_nat count_acc_nat_eq
+HOL_To_IMP_Minus_correct HOL_To_HOL_Nat.count_acc_nat
+  oops
 
-lemma related_zip_nat_unconditional [transfer_rule]:
-  "(Rel_nat ===> Rel_nat ===> Rel_nat) zip_nat_unconditional List.zip"
-  sorry
+lemma count_acc_cor: "Rel_nat (s ''count_acc_nat.args.x'') (y::'a) \<Longrightarrow>
+    Rel_nat (s ''count_acc_nat.args.xa'') (ya::'a list) \<Longrightarrow>
+    Rel_nat (s ''count_acc_nat.args.xb'') (yb::nat) \<Longrightarrow>
+    terminates_with_res_IMP_Minus
+     (tailcall_to_IMP_Minus count_acc_nat_IMP_tailcall) s
+     ''count_acc_nat.ret''
+     (HTHN.count_acc_nat TYPE('a::compile_nat)
+       (s ''count_acc_nat.args.x'')
+       (s ''count_acc_nat.args.xa'')
+       (s ''count_acc_nat.args.xb''))"
+  apply (rule terminates_with_res_IMP_Minus_if_terminates_with_res_IMP_TailcallI)
+   apply (subst count_acc_nat_IMP_tailcall_def; simp)
+   apply (subst count_acc_nat_IMP_tailcall_def; simp)
+  apply (induction y ya yb arbitrary: s rule: HTHN.count_acc.induct)
+  (* case [] *)
+  apply (subst (2) count_acc_nat_IMP_tailcall_def, rule terminates_with_res_IMP_Tailcall_start)
+  apply (tactic \<open>HT.run_step_tac HT.get_imp_minus_correct @{context} 1\<close>)+
+    (* correct case *)
+    apply (subst HTHN.count_acc_nat_eq_unfolded)
+    apply (assumption, assumption, assumption)
+    apply (subst case_list_nat_def)
+    apply (split if_splits; intro impI conjI; simp)
+    apply (tactic \<open>HT.finish_non_tail_tac @{context} 1\<close>)
+    (* wrong case *)
+    apply (erule check_first_nat_ccontradictionE check_first_nat_ccontradictionE')
+    apply (rule fst_nat_eq_if_Rel_nat_list)
+    apply assumption
+    apply simp
+  (* case x#xs *)
+  apply (subst (2) count_acc_nat_IMP_tailcall_def, rule terminates_with_res_IMP_Tailcall_start)
+  apply (tactic \<open>HT.run_step_tac HT.get_imp_minus_correct @{context} 1\<close>)+
+    apply (erule check_first_nat_ccontradictionE check_first_nat_ccontradictionE')
+    apply (rule fst_nat_eq_if_Rel_nat_list)
+    apply assumption
+    apply simp
+  apply (tactic \<open>HT.run_step_tac HT.get_imp_minus_correct @{context} 1\<close>)+
+    apply (subst HTHN.count_acc_nat_eq_unfolded)
+    apply (assumption, assumption, assumption)
+    apply (subst case_list_nat_def)
+    apply (split if_splits; intro impI conjI; simp)
+    subgoal for v
+    sorry
+  apply (tactic \<open>HT.run_step_tac HT.get_imp_minus_correct @{context} 1\<close>)+
+    apply (subst HTHN.count_acc_nat_eq_unfolded)
+    apply (assumption, assumption, assumption)
+    apply (subst case_list_nat_def)
+    apply (split if_splits; intro impI conjI; simp)
+    subgoal for v
+    sorry
+  done
+
+HOL_To_IMP_Minus_correct HOL_To_HOL_Nat.count_acc_nat
+  using count_acc_cor by blast
 
 end
+
+
+context HOL_To_HOL_Nat
+begin
+
+fun count_acc2 :: "'a \<Rightarrow> 'a list \<Rightarrow> nat \<Rightarrow> nat" where
+  "count_acc2 a [] n = n"
+| "count_acc2 a (x#xs) n = count_acc2 a xs (if x = a then Suc n else n)"
+declare count_acc2.simps[simp del]
+
+case_of_simps count_acc2_eq : count_acc2.simps
+function_compile_nat count_acc2_eq
+
+end
+
+context HOL_Nat_To_IMP_Minus
+begin
+
+lemmas count_acc2_nat_eq = HTHN.count_acc2_nat_eq_unfolded[simplified case_list_nat_def]
+compile_nat count_acc2_nat_eq
+HOL_To_IMP_Minus_correct HOL_To_HOL_Nat.count_acc2_nat
+  oops
+
+lemma count_acc2_cor: "Rel_nat (s ''count_acc2_nat.args.x'') (y::'a) \<Longrightarrow>
+    Rel_nat (s ''count_acc2_nat.args.xa'') (ya::'a list) \<Longrightarrow>
+    Rel_nat (s ''count_acc2_nat.args.xb'') (yb::nat) \<Longrightarrow>
+    terminates_with_res_IMP_Minus
+     (tailcall_to_IMP_Minus count_acc2_nat_IMP_tailcall) s
+     ''count_acc2_nat.ret''
+     (HTHN.count_acc2_nat TYPE('a::compile_nat)
+       (s ''count_acc2_nat.args.x'')
+       (s ''count_acc2_nat.args.xa'')
+       (s ''count_acc2_nat.args.xb''))"
+  apply (rule terminates_with_res_IMP_Minus_if_terminates_with_res_IMP_TailcallI)
+   apply (subst count_acc2_nat_IMP_tailcall_def; simp)
+   apply (subst count_acc2_nat_IMP_tailcall_def; simp)
+  apply (induction y ya yb arbitrary: s rule: HTHN.count_acc.induct)
+  (* case [] *)
+  apply (subst (2) count_acc2_nat_IMP_tailcall_def, rule terminates_with_res_IMP_Tailcall_start)
+  apply (tactic \<open>HT.run_step_tac HT.get_imp_minus_correct @{context} 1\<close>)+
+    (* correct case *)
+    apply (subst HTHN.count_acc2_nat_eq_unfolded)
+    apply (assumption, assumption, assumption)
+    apply (subst case_list_nat_def)
+    apply (split if_splits; intro impI conjI; simp)
+    apply (tactic \<open>HT.finish_non_tail_tac @{context} 1\<close>)
+    (* wrong case *)
+    apply (erule check_first_nat_ccontradictionE check_first_nat_ccontradictionE')
+    apply (rule fst_nat_eq_if_Rel_nat_list)
+    apply assumption
+    apply simp
+  (* case x#xs *)
+  apply (subst (2) count_acc2_nat_IMP_tailcall_def, rule terminates_with_res_IMP_Tailcall_start)
+  apply (tactic \<open>HT.run_step_tac HT.get_imp_minus_correct @{context} 1\<close>)+
+    apply (erule check_first_nat_ccontradictionE check_first_nat_ccontradictionE')
+    apply (rule fst_nat_eq_if_Rel_nat_list)
+    apply assumption
+    apply simp
+  apply (tactic \<open>HT.run_step_tac HT.get_imp_minus_correct @{context} 1\<close>)+
+  sorry
+
+HOL_To_IMP_Minus_correct HOL_To_HOL_Nat.count_acc2_nat
+  using count_acc2_cor by blast
+
 
 end
